\documentclass[12pt]{article}
\usepackage{parskip,amsmath,amssymb}
\usepackage[margin=.6in]{geometry}

\begin{document}
\begin{enumerate}
    \item
    \begin{align*}
        (f*g)(t)
        &= \begin{cases}
            \int_{0}^{t}\tau d\tau, & : 0 \leq t < 1\\
            \int_{t-1}^{1}\tau d\tau, & : 1 \leq t  2\\
            \end{cases}\\
        &= \begin{cases}
            \frac{1}{2}\tau^2 |_{0}^{t}, & : 0 \leq t < 1\\
            \frac{1}{2}\tau^2 |_{t-1}^{1}, & : 1 \leq t  2\\
            \end{cases}\\
        &= \begin{cases}
            \frac{1}{2}t^2, & : 0 \leq t < 1\\
            -\frac{1}{2}(t^2 + 2t), & : 1 \leq t  2\\
            \end{cases}\\
        &= \frac{1}{2}t^2 u_{-1}(t) - \frac{1}{2}t^2 u_{-1}(t - 1) + (-\frac{1}{2}t^2 + t)u_{-1}(t-1) - (-\frac{1}{2}t^2 + t)u_{-1}(t-2)\\
    \end{align*}
    \item
    \begin{align*}
        F(S) &= \mathcal{L}\{u_{-1}(t)-u_{1}(t-1)\}\\
        &= \mathcal{L}\{u_{-1}(t)\}-\mathcal{L}\{u_{1}(t-1)\}\\
        &= \frac{1}{s} - \frac{1}{se^s}\\\\
        G(S) &= \mathcal{L}\{t(u_{-1}(t)-u_{1}(t-1))\}\\
        &= -\frac{d}{ds}\mathcal{L}\{u_{-1}(t)-u_{1}(t-1)\}\\
        &=-\frac{d}{ds}(\frac{1}{s} - \frac{1}{se^s})\\
        &= -(\frac{-1}{s^2} - (\frac{-1}{se^s} + \frac{-1}{s^2e^s}))\\
        &= \frac{1}{s^2} - \frac{1}{se^s} - \frac{1}{s^2e^s}
    \end{align*}
    \item
    \begin{align*}
        \mathcal{L} \{(f*g)(t)\} &= \frac{1}{2}\mathcal{L}\{t^2 u_{-1}(t)\} - \frac{1}{2}\mathcal{L}\{t^2 u_{-1}(t-1)\} + -\frac{1}{2}\mathcal{L}\{(t^2 + 2t)u_{-1}(t-1)\} - -\frac{1}{2}\mathcal{L}\{(t^2 + 2t)u_{-1}(t-2)\}\\
        &= \frac{1}{s^3} - \frac{s^2 + 2s + 2}{2s^3e^s} \frac{s^2 + 2s + 2}{2s^3e^s} -\frac{s+1}{s^2e^s} +\frac{2s^2 + 2s + 1}{s^3e^s} + \frac{2s+1}{s^2e^s}
    \end{align*}
    \item The answer for c is the multiplication of the two answers from b
\end{enumerate}


\end{document}
